Last sorry at Clause.consClosed remaining

InferenceInLean/Syntax.lean
@@ -66,7 +66,8 @@ inductive Atom where
 
 @[simp]
 def Atom.freeVars {sig : Signature} {X : Variables} : Atom sig X -> Set X
-  | .pred _ args => args.foldl (fun acc t => acc ∪ Term.freeVars sig X t) ∅
+  | .pred _ [] => ∅
+  | .pred P (a :: args) => a.freeVars ∪ (Atom.pred P args).freeVars
 
 inductive Literal where
   | pos (a : Atom sig X)
@@ -140,14 +141,60 @@ instance : Coe (Clause sig X) (Formula sig X) :=
 instance : Coe (Set <| Clause sig X) (Set <| Formula sig X) :=
   ⟨fun N => {↑C | C ∈ N}⟩
 
-def Term.freeVarsList : Term sig X -> List X
+@[simp]
+def Term.freeVarsList [DecidableEq X] : Term sig X -> List X
   | Term.var x => [x]
   | Term.func _ [] => []
-  | Term.func f (a :: args) => (Term.freeVarsList a).append (Term.freeVarsList (Term.func f args))
+  | Term.func f (a :: args) => List.dedup ((Term.freeVarsList a).append (Term.freeVarsList (Term.func f args)))
+
+@[simp]
+lemma Term.freeVars_sub_freeVarsList [DecidableEq X] (t : Term sig X) :
+    t.freeVars ⊆ (t.freeVarsList).toFinset := by
+  induction' t using Term.induction with x args ih f
+  · aesop
+  · induction args with
+    | nil => aesop
+    | cons head tail ih' =>
+      simp
+      constructor
+      · specialize ih head (by simp)
+        generalize freeVarsList sig X head = Fl at *
+        generalize freeVars sig X head = Fs at *
+        intro x hxinFs
+        simp only [Set.mem_setOf_eq]
+        left
+        exact List.mem_dedup.mp (ih hxinFs)
+      · simp_all only [List.coe_toFinset]
+        intro x hxinfree
+        aesop
 
 def Atom.freeVarsList [DecidableEq X] : Atom sig X -> List X
   | .pred _ [] => []
   | .pred P (t :: ts) => List.dedup ((t.freeVarsList).append (Atom.pred P ts).freeVarsList)
+
+def Atom.freeVars_sub_freeVarsList [DecidableEq X] (a : Atom sig X) :
+    a.freeVars ⊆ (a.freeVarsList).toFinset := by
+  simp_all only [List.coe_toFinset]
+  induction a with
+  | pred p args =>
+    induction args with
+    | nil => aesop
+    | cons head tail ih =>
+      simp only [freeVars, Set.union_subset_iff]
+      constructor
+      · have hfree_subset := Term.freeVars_sub_freeVarsList sig X head
+        unfold freeVarsList
+        intro x hxinfree
+        simp_all only [List.coe_toFinset, List.append_eq, List.mem_dedup, List.mem_append, Set.mem_setOf_eq]
+        apply Or.inl
+        apply hfree_subset
+        simp_all only
+      · unfold freeVarsList
+        intro x hxinfree
+        simp_all only [List.coe_toFinset, List.append_eq, List.mem_dedup, List.mem_append, Set.mem_setOf_eq]
+        apply Or.inr
+        apply ih
+        exact hxinfree
 
 def Clause.freeVarsList [DecidableEq X] : Clause sig X -> List X
   | [] => []
@@ -155,21 +202,31 @@ def Clause.freeVarsList [DecidableEq X] : Clause sig X -> List X
   | (.neg l) :: ls => List.dedup (l.freeVarsList ++ freeVarsList ls)
 
 @[simp]
-def Clause.toClosedFormula [DecidableEq X] (C : Clause sig X) : Formula sig X :=
-  Formula.bigForall sig X (C.freeVarsList) C
-
-theorem Clause.closedClause_closed [DecidableEq X] (C : Clause sig X) :
-    Formula.closed C.toClosedFormula := by
-  unfold toClosedFormula
-  unfold Formula.closed
-  unfold Formula.freeVars
-  sorry
-
-theorem nodup_clauseFreeVarsList [DecidableEq X] (C : Clause sig X) :
+lemma nodup_clauseFreeVarsList [DecidableEq X] (C : Clause sig X) :
     List.Nodup (C.freeVarsList) := by
   unfold Clause.freeVarsList
   simp_all only [Clause]
   split <;> simp_all only [List.nodup_nil, List.nodup_dedup]
+
+@[simp]
+def Clause.toClosedFormula [DecidableEq X] (C : Clause sig X) : Formula sig X :=
+  Formula.bigForall sig X (C.freeVarsList) C
+
+lemma Clause.closedEmpty_closed [DecidableEq X] :
+    Formula.closed (Clause.toClosedFormula sig X []) := by aesop
+
+lemma Clause.consClosed [DecidableEq X] (L : Literal sig X) (C : Clause sig X) :
+    (Clause.toClosedFormula sig X C).closed → (Clause.toClosedFormula sig X (L :: C)).closed := by
+  intro h
+  sorry
+
+theorem Clause.closedClause_closed [DecidableEq X] (C : Clause sig X) :
+    Formula.closed C.toClosedFormula := by
+  induction C with
+  | nil => aesop
+  | cons head tail ih =>
+    simp_all
+    exact Clause.consClosed sig X head tail ih
 
 @[simp]
 def Substitution := X -> Term sig X
